Implement pattern compilation (no termination), prove dispatch equiv
Implement full compilation function
Termination is tricky, need to prove (with Equations)
Implemented both versions of dispatch, proved equivalence

proofs/core/Pattern.v
@@ -1,56 +1,192 @@
 (*Compilation of pattern matches*)
 Require Import Syntax Denotational.
+Set Bullet Behavior "Strict Subproofs".
+From Equations Require Import Equations.
 
 (*TODO: don't really need but matches interface*)
 Definition amap_change {A B: Type} (eq_dec: forall (x y: A), {x = y} + { x <> y}) 
   (f: option B -> B) (x: A) (m: amap A B) : amap A B :=
   amap_replace eq_dec m x (fun _ b => f (Some b)) (f None).
-Print amap.
-Definition amap_map {A B C: Type} (f: B -> C) (m: amap A B) : amap B C :=
-
 
 Section Compile.
 Context {A: Type} (get_constructors: typesym -> list funsym) 
-  (mk_case: term -> list (pattern * A)) (mk_let: vsymbol -> term -> A -> A).
+  (mk_case: term -> list (pattern * A) -> A) (mk_let: vsymbol -> term -> A -> A).
 
-(*NOTE: several different notions of simplification/dispatch, prove equivalent*)
-
-(*Not having maps is annoying*)
-Check get_assoc_list.
-Check amap.
-Definition dispatch :=
-  let add_case fs pl a (cases : amap funsym (list (list pattern * A))) :=
+(*We separate out some helper functions*)
+Definition add_case (fs: funsym) (pl: list pattern) (a: A) (cases : amap funsym (list (list pattern * A))) :=
     amap_change funsym_eq_dec (fun o =>
       match o with
       | None => [(pl, a)]
       | Some rl => (pl, a) :: rl
       end
-      ) fs cases
-  in
-  let union_cases pl a types cases :=
+    ) fs cases.
+
+Definition union_cases (pl: list pattern) (a: A) (types: amap funsym (list pattern)) 
+    (cases: amap funsym (list (list pattern * A))) : amap funsym (list (list pattern * A)) :=
     let add pl _ := Pwild :: pl in
     let wild ql := [(fold_left add ql pl, a)] in
     let join _ wl rl := Some (wl ++ rl) in
-    amap_union join (amap_map wild types) cases 
-  in
+    amap_union funsym_eq_dec join (amap_map wild types) cases .
+
+(*Part 1: The dispatch function they implement in OCaml
+  This is more efficient (1 pass) but harder to directly reason about*)
+
+(*The induction is non-trivial - we recurse inside the pattern.
+  We will need a version of this later for terms as well*)
+Fixpoint pat_size (p: pattern) : nat :=
+  match p with
+  | Por p1 p2 => 1 + pat_size p1 + pat_size p2
+  | Pbind p _ => 1 + pat_size p
+  | Pconstr _ _ ps => 1 + sum (map pat_size ps)
+  | _ => 1
+  end.
+Definition pat_list_size (l: list pattern) : nat :=
+  sum (map pat_size l).
+Lemma pat_list_size_cons p l :
+  pat_list_size (p :: l) = pat_size p + pat_list_size l.
+Proof.
+  reflexivity.
+Qed.
+
+Section Dispatch.
+Variable (t: term) (types: amap funsym (list pattern)) .
+Equations dispatch (x: list pattern * A) 
+  (y:  (amap funsym (list (list pattern * A))) * list (list pattern * A) ) : 
+  (amap funsym (list (list pattern * A))) * list (list pattern * A) 
+  by wf (pat_list_size (fst x)) lt  :=
+  dispatch (nil, _) y := (*impossible*) (amap_empty, nil);
+  dispatch (Pvar x :: pl, a) (cases, wilds) := 
+    let a := mk_let x t a in
+    (union_cases pl a types cases, (pl, a) :: wilds);
+  dispatch (Pconstr fs _ pl' :: pl, a) (cases, wilds) :=
+    (add_case fs (rev pl' ++ pl) a cases, wilds);
+  dispatch (Pwild :: pl, a) (cases, wilds) :=
+    (union_cases pl a types cases, (pl, a) :: wilds);
+  dispatch (Por p q :: pl, a) (cases, wilds) :=
+    dispatch (p :: pl, a) (dispatch (q :: pl, a) (cases, wilds));
+  dispatch (Pbind p x :: pl, a) (cases, wilds) :=
+    dispatch (p :: pl, mk_let x t a) (cases, wilds).
+Next Obligation.
+  rewrite !pat_list_size_cons. simpl. lia.
+Defined.
+Next Obligation.
+  rewrite !pat_list_size_cons. simpl. lia.
+Defined.
+
+Definition dispatch1 rl := fold_right dispatch (amap_empty, nil) rl.
+
+(*Part 2: An alternative that takes 2 stages: remove all var/bind/or patterns, 
+  and then build map. This is structurally recursive and easier to reason about*)
+Fixpoint simplify_aux (a: A) (p: pattern) : list (pattern * A) :=
+  match p with
+  | Pbind p1 x => (*map (fun '(p2, y) => (p2, mk_let x t y))*) (simplify_aux (mk_let x t a) p1)
+  | Por p1 p2 => simplify_aux a p1 ++ simplify_aux a p2
+  | Pvar x => [(Pwild, mk_let x t a)]
+  | _ => [(p, a)]
+  end.
+
+Definition simplify_single (x: list pattern * A) : list (list pattern * A) :=
+  let (ps, a) := x in
+  let p := List.hd Pwild ps in
+    let ptl := List.tl ps in
+    map (fun '(p1, y) => (p1 :: ptl, y)) (simplify_aux a p).
+
+Definition simplify (rl: list (list pattern * A)) : list (list pattern * A) :=
+  concat (map simplify_single rl).
+
+Definition dispatch2_aux (x: list pattern * A) 
+  (y:  (amap funsym (list (list pattern * A))) * list (list pattern * A) ) : 
+  (amap funsym (list (list pattern * A))) * list (list pattern * A) :=
+  let (pl, a) := x in
+  let (cases, wilds) := y in
+  let p := List.hd Pwild pl in
+  let pl := List.tl pl in
+  match p with
+  | Pconstr fs _ pl' => (add_case fs (rev pl' ++ pl) a cases, wilds)
+  | Pwild => (union_cases pl a types cases, (pl, a) :: wilds)
+  | _ => (*impossible*) (cases, wilds)
+  end.
+
+Definition dispatch2 (rl: list (list pattern * A)) :
+  amap funsym (list (list pattern * A)) * list (list pattern * A) :=
+  fold_right dispatch2_aux (amap_empty, nil) (simplify rl).
+
+(*We need this for the odd induction principle*)
+Lemma dispatch_equiv_aux x base 
+  (Hnull: negb (null (fst x))):
+  dispatch x base =
+  fold_right dispatch2_aux base (simplify_single x).
+Proof.
+  revert x base Hnull.
+  apply (dispatch_elim (fun x base rec => negb (null (fst x)) -> 
+    rec = fold_right dispatch2_aux base (simplify_single x))); auto.
+  - intros. discriminate.
+  - intros p q pl a cases wilds IH1 IH2. simpl in *.
+    intros _.
+    rewrite map_app, fold_right_app.
+    rewrite <- IH1; auto.
+Qed.
+ 
+(*Now we prove equivalence*)
+Lemma dispatch_equiv rl (Hrl: Forall (fun x => negb (null (fst x))) rl):
+  dispatch1 rl = dispatch2 rl.
+Proof.
+  unfold dispatch2, dispatch1.
+  induction rl as [|[pl a] ps IH]; simpl; auto.
+  inversion Hrl as [|? ? Hpl Hps]; subst; simpl in *.
+  unfold simplify in *. simpl.
+  rewrite fold_right_app.
+  destruct pl as [| phd ptl]; simpl in *; try discriminate.
+  rewrite <- IH; auto.
+  destruct (fold_right dispatch (amap_empty, []) ps) as [cases1 wilds1] eqn : Hd2.
+  apply dispatch_equiv_aux. reflexivity.
+Qed.
+End Dispatch.
+
+(*Now define full compilation*)
+Require Import GenElts.
+Check gen_vars.
+
+Definition rev_map {B C: Type} (f: B -> C) (l: list B) : list C :=
+  rev (map f l).
 
 
+Fixpoint fold_left_opt {B C: Type} (f: B -> C -> option B) (l: list C) (base: B) : option B :=
+  match l with
+  | nil => Some base
+  | x :: xs =>
+    match (f base x) with
+    | None => None
+    | Some y => fold_left_opt f xs y
+    end
+  end.
+  
+(*Measure: total term size*)
+(* We can be very permissive here*)
+Fixpoint term_size (t: term) : nat :=
+  match t with
+  | Tfun _ _ ts => 1 + sum (map term_size ts)
+  | _ => 1
+  end.
 
-
-
-    amap_replace funsym_eq_dec cases fs (fun )
-
-
-
-
-Definition simplify_dispatch
+Definition term_list_size (l: list term) : nat :=
+  sum (map term_size l).
 
 (*None = NonExhaustive*)
-Fixpoint compile (tl: list (term * vty)) (rl: list (list pattern * A)) : option A :=
-  match tl, rl with
+
+Definition compile_size (l: list (list pattern * A)) : nat :=
+  sum (map pat_list_size (map fst l)).
+
+(*NOTE: will try to do with pattern, I think that is terminating*)
+Equations compile (tl: list (term * vty)) (rl: list (list pattern * A)) : option A 
+  by wf (compile_size rl) lt :=
+  compile _ [] := None;
+  compile [] ((_, a) :: _) => Some a;
+  compile ((t, ty) :: tl) rl =>
+  (* match tl, rl with
   | _, [] => None
   | nil, (_, a) :: _ => Some a
-  | (t, ty) :: tl, _ =>
+  | (t, ty) :: tl, _ => *)
     (*No bare*)
     (*extarct the set of constructors*)
     let css :=
@@ -65,29 +201,95 @@ Fixpoint compile (tl: list (term * vty)) (rl: list (list pattern * A)) : option 
 
     (*Map every constructor ocurring at the head of the pattern list to the
       list of its args*)
-    let types :=
+    let (types, cslist) :=
       (*NOTE: we don't have maps, not ideal*)
-      let fix populate (acc : list (funsym * list pattern)) 
-        (p: pattern) : list (funsym * list pattern) :=
+      let fix populate (acc : amap funsym (list pattern) * list (funsym * list vty * list pattern)) 
+        (p: pattern) : amap funsym (list pattern) * list (funsym * list vty * list pattern) :=
         match p with
         | Pwild => acc
         | Pvar _ => acc
-        | Pconstr fs _ ps => if is_constr fs then
-            if in_bool funsym_eq_dec fs (map fst acc) then acc else
-            (fs, ps) :: acc
-          else nil (*impossible case - Why3 throws exception here*)
+        | Pconstr fs params ps =>
+          let (css, csl) := acc in
+            if is_constr fs then
+            if amap_mem funsym_eq_dec fs css then acc else
+            (amap_set funsym_eq_dec css fs ps, (fs, params, ps) :: csl)
+          else acc (*impossible case - Why3 throws exception here*)
         | Por p1 p2 => populate (populate acc p1) p2
         | Pbind p _ => populate acc p
         end
       in
-      fold_left populate (map (fun x => List.hd Pwild (fst x)) rl) nil 
+      fold_left populate (map (fun x => List.hd Pwild (fst x)) rl) (amap_empty, nil) 
     in 
     
     (*dispatch part*)
+    let (cases, wilds) := dispatch1 t types rl in
 
+    let comp_cases cs (al : list (term * vty)) :=
+      let l := match (amap_get funsym_eq_dec cases cs ) with
+      | None => nil (*impossible*)
+      | Some l => l
+      end in
+      compile (rev al ++ tl) l in
+
+    let comp_wilds (_: unit) := compile tl wilds in 
+
+    (*TODO: default case here*)
+    let comp_full (_: unit) :=
+      let no_wilds := forallb (fun f => amap_mem funsym_eq_dec f types) css in
+      let base : option (list (pattern * A)) := if no_wilds then Some nil else (*TODO: bind*)
+       match comp_wilds tt with
+        | None => None
+        | Some x => Some [(Pwild, x)]
+      end in
+
+      let add acc (x: funsym * list vty * list pattern) : option (list (pattern * A)) :=
+        let '(cs, params, ql) := x in
+        (*create variables*)
+        let pat_tys :=  (map (ty_subst (s_params cs) params) (s_args cs)) in
+        let new_var_names := gen_vars (length ql) (tm_fv t ++ tm_bnd t) in
+        let typed_vars := map (fun '(x, y) => (fst x, y)) (combine new_var_names pat_tys) in
+        let vl := rev typed_vars in 
+        (*rev_map (fun x => 
+          let v := fst x in
+          let p := fst (snd x) in
+          let ty := snd (snd x) in
+          (fst v, ty)) (combine new_var_names ql) in*)
+        let pl := rev_map Pvar vl in
+        let al := rev_map Tvar vl in
+        match (comp_cases cs (combine al (map snd vl))) with
+        | None => None
+        | Some v => Some ((Pconstr cs params pl, v) :: acc)
+        end
+      in
+      (*TODO: bind*)
+      match base with
+      | None => None
+      | Some b =>
+        match (fold_left_opt add cslist b) with
+        | None => None
+        | Some b1 => Some (mk_case t b1)
+        end
+      end in 
     
+    if null (proj1_sig types) (*TODO: abstraction*) then comp_wilds tt
+    else
     
-    
-    compile tl rl
-    
-  end.
+    match t with
+    | Tfun cs params al =>
+      if is_constr cs then
+        if amap_mem funsym_eq_dec cs types then comp_cases cs (combine al
+          (map (ty_subst (s_params cs) params) (s_args cs))) else comp_wilds tt
+      else comp_full tt
+    | _ => 
+      comp_full tt 
+    end.
+Next Obligation.
+(*Problem: lose information about cases here*)
+
+(*Idea:
+  1. Prove that everything in cases has compile_size smaller than rl
+  2. Prove that wilds has size smaller than rl 
+  3. Probably (maybe) need to inline comp_cases/comp_wilds, or make dependently typed
+    may need some kind of convoy pattern so that Equations knows where cases comes from*)
+
+  (*          let pat_tys := (map (ty_subst (s_params fs) params) (s_args fs)) in*)
